New dependent S typing: basic identity works

formal/SkLean/Checker.lean
@@ -3,12 +3,14 @@ import SkLean.Eval
 
 inductive TypeError {α : Type} where
   | argument_mismatch (expected actual in_e arg : α) : TypeError
-  | no_type_not_comb  (at_e : α)                 : TypeError
+  | no_type_not_comb  (at_e : α)                     : TypeError
+  | bad_type_not_comb (at_e t : α)                   : TypeError
 
 instance (α : Type) [ToString α] : ToString (@TypeError α) where
   toString
   | .argument_mismatch expected actual in_e arg => s!"Argument type mismatch in function application of {in_e} with {arg}. Expected {expected}, but found {actual}"
-  | .no_type_not_comb at_e => s!"type inference failed for {at_e}, but not a combinator"
+  | .no_type_not_comb at_e => s!"Type inference failed for {at_e}, but not a combinator."
+  | .bad_type_not_comb t at_e => s!"Type inference failed for {at_e}. Expected an arrow, but got {t}, but not a combinator."
 
 namespace Expr
 
@@ -26,6 +28,7 @@ def is_typed_comb : Ast.Expr → Bool
 
 def add_m : Ast.Expr → Ast.Expr
   | SKM[M]    => SKM[(M M)]
+  | SKM[_]    => SKM[(M _)]
   | SKM[K]    => SKM[(M K)]
   | SKM[S]    => SKM[(M S)]
   | SKM[#~>]  => SKM[(M #~>)]
@@ -33,7 +36,7 @@ def add_m : Ast.Expr → Ast.Expr
   | SKM[Prp]  => SKM[(M Prp)]
   | SKM[(lhs rhs)] => SKM[((#(add_m lhs)) rhs)]
 
-def infer : Ast.Expr → Except (@TypeError Ast.Expr) Ast.Expr
+partial def infer_unsafe : Ast.Expr → Except (@TypeError Ast.Expr) Ast.Expr
   | SKM[K]               => pure SKM[(M K)]
   | SKM[S]               => pure SKM[(M S)]
   | SKM[M]               => pure SKM[(M M)]
@@ -43,38 +46,50 @@ def infer : Ast.Expr → Except (@TypeError Ast.Expr) Ast.Expr
   | SKM[(M M)]           => pure SKM[Prp]
   | SKM[(M #~>)]         => pure SKM[Prp]
   | SKM[Prp]             => pure SKM[Ty 0]
+  | SKM[_]               => .error $ .no_type_not_comb SKM[_]
   | SKM[Ty n]            => pure SKM[Ty n.succ]
-  | SKM[((K α) β)]       => pure SKM[(α ~> (((K (Ty 0)) α) (β ~> (((K (M β)) α) β))))]
-  | SKM[(((S α) β) γ)]   => pure SKM[(α ~> ((((K (Ty 0))) α) (β ~> ((((K (Ty 0)) β) (γ ~> (((((S (M α)) (M β)) γ) α) β)))))))]
-  | SKM[(M e)] => do pure SKM[(M #(← infer e))]
+  | SKM[((K α) β)]       => pure SKM[α !~> β !~> α]
+  | SKM[(((K _) β) x)]   => do
+    let α ← infer_unsafe x
+    pure SKM[α !~> β !~> α]
+  | SKM[(((S α) β) γ)]   => do
+    let t_α ← infer_unsafe α
+    pure $ Ast.Expr.mk_s_type t_α α β γ
+  | SKM[(((((S α) _) γ) _x) y)]   => do
+    let β ← infer_unsafe y
+    let t_α ← infer_unsafe α
+    pure $ Ast.Expr.mk_s_type t_α α β γ
+  | SKM[(M e)] => do pure SKM[(M #(← infer_unsafe e))]
   | SKM[(_t_in ~> _t_out)] => pure SKM[Ty 0]
   | SKM[(lhs rhs)]       => do
-    let t_lhs ← infer lhs
-    match (eval_once t_lhs).getD t_lhs with
+    let t_lhs ← infer_unsafe lhs
+    let t_lhs' := (eval_unsafe t_lhs).getD t_lhs
+
+    match t_lhs' with
     | SKM[(t_in ~> _t_out)] =>
-      let found ← infer rhs
+      let found ← infer_unsafe rhs
 
       if found == t_in then
-        pure $ (eval_once SKM[(t_lhs rhs)]).getD SKM[(t_lhs rhs)]
+        pure $ (eval_unsafe SKM[(t_lhs' rhs)]).getD SKM[(t_lhs rhs)]
       else
         .error $ .argument_mismatch t_in t_lhs lhs rhs
     | e =>
       if is_typed_comb e then
         let with_m := SKM[((#(add_m lhs)) rhs)]
-        pure $ (eval_once with_m).getD with_m
+        pure $ (eval_unsafe with_m).getD with_m
       else
-        .error $ .no_type_not_comb lhs
+        .error $ .bad_type_not_comb lhs t_lhs'
 
-lemma valid_lhs (_h_t : infer SKM[(lhs rhs)] = .ok t) : ∃ t_lhs, infer lhs = t_lhs := by
+lemma valid_lhs (_h_t : infer_unsafe SKM[(lhs rhs)] = .ok t) : ∃ t_lhs, infer_unsafe lhs = t_lhs := by
   cases SKM[(lhs rhs)]
   repeat simp_all
 
-lemma valid_rhs (_h_t : infer SKM[(lhs rhs)] = .ok t) : ∃ t_rhs, infer rhs = t_rhs := by
+lemma valid_rhs (_h_t : infer_unsafe SKM[(lhs rhs)] = .ok t) : ∃ t_rhs, infer_unsafe rhs = t_rhs := by
   cases SKM[(lhs rhs)]
   repeat simp_all
 
 end Expr
 
-#eval Expr.infer SKM[((((K (M K)) (M K)) K) K)]
+#eval Expr.infer_unsafe SKM[((((K (M K)) (M K)) K) K)]
 
-example : Expr.infer SKM[((((K (M K)) (M K)) K) K)] = .ok SKM[(M K)] := rfl
+#eval Expr.infer_unsafe SKM[((((((S (Ty 0 !~> (Ty 0 !~> Ty 0) !~> Ty 0)) (Ty 0 !~> Ty 0 !~> Ty 0)) Ty 0) ((K Ty 0) (Ty 0 !~> Ty 0))) ((K Ty 0) Ty 0)) Prp)]
