formal/SkLean/Ast3.lean
@@ -9,6 +9,7 @@ inductive Expr where
   | m    : Expr
   | arr  : Expr
   | prp  : Expr
+  | hole : Expr
   | ty   : ℕ    → Expr
   | call : Expr → Expr → Expr
 deriving BEq, Repr, Lean.ToExpr
@@ -24,6 +25,7 @@ syntax "Prp"                   : skmexpr
 syntax "Ty" term               : skmexpr
 syntax "Typ" num               : skmexpr
 syntax "#~>"                   : skmexpr
+syntax "_"                     : skmexpr
 syntax skmexpr "~>" skmexpr    : skmexpr
 syntax skmexpr "!~>" skmexpr   : skmexpr
 syntax "(" skmexpr skmexpr ")" : skmexpr
@@ -44,6 +46,7 @@ macro_rules
   | `(⟪ Prp ⟫)                         => `(Expr.prp)
   | `(⟪ Ty $n:term ⟫)                  => `(Expr.ty $n)
   | `(⟪ Typ $n:num ⟫)                  => `(Expr.ty $n)
+  | `(⟪ _ ⟫)                           => `(Expr.hole)
   | `(⟪ #~> ⟫)                         => `(Expr.arr)
   | `(⟪ $e₁:skmexpr !~> $e₂:skmexpr ⟫) => `(SKM[$e₁ ~> (((K (Ty 0)) $e₁) $e₂)])
   | `(⟪ $e₁:skmexpr ~> $e₂:skmexpr ⟫)  => `(Expr.call (Expr.call Expr.arr ⟪ $e₁ ⟫) ⟪ $e₂ ⟫)
@@ -59,11 +62,16 @@ def toStringImpl (e : Expr) : String :=
   | SKM[S]    => "S"
   | SKM[K]    => "K"
   | SKM[M]    => "M"
+  | SKM[_]    => "_"
   | SKM[#~>]  => "→"
   | SKM[Ty n] => s!"Type {n}"
   | SKM[Prp]  => "Prop"
-  | SKM[((t_in ~> t_out) ~> t₃)] => s!"({t_in.toStringImpl} → {t_out.toStringImpl}) → {t₃.toStringImpl}"
-  | SKM[(t_in ~> t_out)] => s!"{t_in.toStringImpl} → {t_out.toStringImpl}"
+  | SKM[(t_in ~> (((K (Ty 0)) t_in') t_out))] =>
+    if t_in' == t_in then
+      s!"({t_in.toStringImpl} !→ {t_out.toStringImpl})"
+    else
+      s!"({t_in.toStringImpl} → {t_out.toStringImpl})"
+  | SKM[(t_in ~> t_out)] => s!"({t_in.toStringImpl} → {t_out.toStringImpl})"
   | SKM[(lhs rhs)] => s!"({lhs.toStringImpl} {rhs.toStringImpl})"
 
 instance : ToString Expr where
@@ -71,9 +79,10 @@ instance : ToString Expr where
 
 def fromExpr (e : Lean.Expr) : Option Expr :=
   match e with
-  | .const `Expr.k [] => pure SKM[K]
-  | .const `Expr.s [] => pure SKM[S]
-  | .const `Expr.m [] => pure SKM[M]
+  | .const `Expr.hole [] => pure SKM[_]
+  | .const `Expr.k []    => pure SKM[K]
+  | .const `Expr.s []    => pure SKM[S]
+  | .const `Expr.m []    => pure SKM[M]
   | .const `Expr.arr [] => pure SKM[#~>]
   | .sort .zero => pure SKM[Prp]
   | .sort n => pure SKM[Ty n.depth.pred]
@@ -82,6 +91,9 @@ def fromExpr (e : Lean.Expr) : Option Expr :=
     let rhs' ← fromExpr rhs
     pure SKM[(lhs' rhs')]
   | _ => none
+
+def mk_s_type (t_α α β γ : Ast.Expr) : Ast.Expr :=
+  SKM[(α !~> β ~> (((((S _) _) β) (((K ((M #~>) γ)) β) (#~> γ))) ((((S t_α) β) γ) α)))]
 
 end Expr
 
